Slightly cleaned up use of variables in typechecking

02Typed/Typechecking.thy
@@ -2,44 +2,65 @@ theory Typechecking
   imports TypedLanguage UnifiableType
 begin
 
+subsection \<open>Typechecking\<close>
+
+text \<open>Now, we can finally define typechecking. The main \<open>typecheck'\<close> function is given a typing 
+context*, a set of already-used variables, and an expression to check, and returns the expression 
+annotated with fresh type variables on each binder, a unifiable term representing the type of the 
+expression, a set of additional used variables, and a constraint that must be unified to establish 
+the final form of the type of the expression. Rather than explicitly failing if we reach an unbound 
+variable, we simply throw an un-unifiable constraint in and fail later.\<close>
+
+text \<open>*The first argument is a \<open>subst\<close> rather than a \<open>var \<rightharpoonup> ty\<close> or \<open>ty list\<close>, but we call it \<Gamma> 
+rather than \<sigma> to emphasize its role as a context in which we look up types, not a substitution we 
+apply to terms.\<close>
+
 primrec typecheck' :: "subst \<Rightarrow> var set \<Rightarrow> 'a expr\<^sub>s \<Rightarrow> uterm expr\<^sub>s \<times> uterm \<times> var set \<times> constraint" 
     where
   "typecheck' \<Gamma> vs (Var\<^sub>s x) = (case \<Gamma> x of 
-      Some t \<Rightarrow> (Var\<^sub>s x, t, vs, []) 
-    | None \<Rightarrow> (Var\<^sub>s x, Num\<^sub>\<tau>, vs, fail))"
-| "typecheck' \<Gamma> vs (Const\<^sub>s k) = (Const\<^sub>s k, Num\<^sub>\<tau>, vs, [])"
-| "typecheck' \<Gamma> vs (Lam\<^sub>s x t e) = (
+      Some \<tau> \<Rightarrow> (Var\<^sub>s x, \<tau>, {}, []) 
+    | None \<Rightarrow> (Var\<^sub>s x, Num\<^sub>\<tau>, {}, fail))"
+| "typecheck' \<Gamma> vs (Const\<^sub>s n) = (Const\<^sub>s n, Num\<^sub>\<tau>, {}, [])"
+| "typecheck' \<Gamma> vs (Lam\<^sub>s x u e) = (
     let v = fresh vs
-    in let (e', t, vs', con) = typecheck' (\<Gamma>(x \<mapsto> Var v)) (insert v vs) e
-    in (Lam\<^sub>s x (Var v) e', Arrow\<^sub>\<tau> (Var v) t, vs', con))"
+    in let (e', \<tau>, vs', \<kappa>) = typecheck' (\<Gamma>(x \<mapsto> Var v)) (insert v vs) e
+    in (Lam\<^sub>s x (Var v) e', Arrow\<^sub>\<tau> (Var v) \<tau>, insert v vs', \<kappa>))"
 | "typecheck' \<Gamma> vs (App\<^sub>s e\<^sub>1 e\<^sub>2) = (
     let v = fresh vs
-    in let (e\<^sub>1', t\<^sub>1, vs', con\<^sub>1) = typecheck' \<Gamma> (insert v vs) e\<^sub>1 
-    in let (e\<^sub>2', t\<^sub>2, vs'', con\<^sub>2) = typecheck' \<Gamma> vs' e\<^sub>2 
-    in (App\<^sub>s e\<^sub>1' e\<^sub>2', Var v, vs'', con\<^sub>1 @ con\<^sub>2 @ [(t\<^sub>1, Arrow\<^sub>\<tau> t\<^sub>2 (Var v))]))"
+    in let (e\<^sub>1', \<tau>\<^sub>1, vs\<^sub>1, \<kappa>\<^sub>1) = typecheck' \<Gamma> (insert v vs) e\<^sub>1 
+    in let (e\<^sub>2', \<tau>\<^sub>2, vs\<^sub>2, \<kappa>\<^sub>2) = typecheck' \<Gamma> (insert v (vs \<union> vs\<^sub>1)) e\<^sub>2 
+    in (App\<^sub>s e\<^sub>1' e\<^sub>2', Var v, insert v (vs\<^sub>1 \<union> vs\<^sub>2), \<kappa>\<^sub>1 @ \<kappa>\<^sub>2 @ [(\<tau>\<^sub>1, Arrow\<^sub>\<tau> \<tau>\<^sub>2 (Var v))]))"
+
+text \<open>As with the unification algorithm, we create an induction method tailored to \<open>typecheck'\<close>.\<close>
 
 lemma typecheck_induct [consumes 1, case_names Var\<^sub>sS Var\<^sub>sN Const\<^sub>s Lam\<^sub>s App\<^sub>s]: "
   typecheck' \<Gamma> vs e = (e', t, vs', con) \<Longrightarrow> 
-  (\<And>\<Gamma> vs t x. \<Gamma> x = Some t \<Longrightarrow> P \<Gamma> vs (Var\<^sub>s x) (Var\<^sub>s x) t vs []) \<Longrightarrow> 
-  (\<And>\<Gamma> vs x. \<Gamma> x = None \<Longrightarrow> P \<Gamma> vs (Var\<^sub>s x) (Var\<^sub>s x) Num\<^sub>\<tau> vs fail) \<Longrightarrow> 
-  (\<And>\<Gamma> vs k. P \<Gamma> vs (Const\<^sub>s k) (Const\<^sub>s k) Num\<^sub>\<tau> vs []) \<Longrightarrow> 
+  (\<And>\<Gamma> vs t x. \<Gamma> x = Some t \<Longrightarrow> P \<Gamma> vs (Var\<^sub>s x) (Var\<^sub>s x) t {} []) \<Longrightarrow> 
+  (\<And>\<Gamma> vs x. \<Gamma> x = None \<Longrightarrow> P \<Gamma> vs (Var\<^sub>s x) (Var\<^sub>s x) Num\<^sub>\<tau> {} fail) \<Longrightarrow> 
+  (\<And>\<Gamma> vs k. P \<Gamma> vs (Const\<^sub>s k) (Const\<^sub>s k) Num\<^sub>\<tau> {} []) \<Longrightarrow> 
   (\<And>\<Gamma> vs vs' con x u e\<^sub>1 e\<^sub>1' t' v. v = fresh vs \<Longrightarrow> typecheck' (\<Gamma>(x \<mapsto> Var v)) (insert v vs) e\<^sub>1 = 
     (e\<^sub>1', t', vs', con) \<Longrightarrow> P (\<Gamma>(x \<mapsto> Var v)) (insert v vs) e\<^sub>1 e\<^sub>1' t' vs' con \<Longrightarrow> 
-      P \<Gamma> vs (Lam\<^sub>s x u e\<^sub>1) (Lam\<^sub>s x (Var v) e\<^sub>1') (Arrow\<^sub>\<tau> (Var v) t') vs' con) \<Longrightarrow> 
+    P \<Gamma> vs (Lam\<^sub>s x u e\<^sub>1) (Lam\<^sub>s x (Var v) e\<^sub>1') (Arrow\<^sub>\<tau> (Var v) t') (insert v vs') con) \<Longrightarrow> 
   (\<And>\<Gamma> vs vs' e\<^sub>1 e\<^sub>2 v e\<^sub>1' t\<^sub>1 vs'' con\<^sub>1 e\<^sub>2' t\<^sub>2 con\<^sub>2. v = fresh vs \<Longrightarrow> 
-    typecheck' \<Gamma> (insert v vs) e\<^sub>1 = (e\<^sub>1', t\<^sub>1, vs'', con\<^sub>1) \<Longrightarrow> 
-      typecheck' \<Gamma> vs'' e\<^sub>2 = (e\<^sub>2', t\<^sub>2, vs', con\<^sub>2) \<Longrightarrow> P \<Gamma> (insert v vs) e\<^sub>1 e\<^sub>1' t\<^sub>1 vs'' con\<^sub>1 \<Longrightarrow> 
-        P \<Gamma> vs'' e\<^sub>2 e\<^sub>2' t\<^sub>2 vs' con\<^sub>2 \<Longrightarrow> P \<Gamma> vs (App\<^sub>s e\<^sub>1 e\<^sub>2) (App\<^sub>s e\<^sub>1' e\<^sub>2') (Var v) vs' 
-          (con\<^sub>1 @ con\<^sub>2 @ [(t\<^sub>1, Arrow\<^sub>\<tau> t\<^sub>2 (Var v))])) \<Longrightarrow> 
-    P \<Gamma> vs e e' t vs' con"
+    typecheck' \<Gamma> (insert v vs) e\<^sub>1 = (e\<^sub>1', t\<^sub>1, vs', con\<^sub>1) \<Longrightarrow> 
+    typecheck' \<Gamma> (insert v (vs \<union> vs')) e\<^sub>2 = (e\<^sub>2', t\<^sub>2, vs'', con\<^sub>2) \<Longrightarrow> 
+    P \<Gamma> (insert v vs) e\<^sub>1 e\<^sub>1' t\<^sub>1 vs' con\<^sub>1 \<Longrightarrow> 
+    P \<Gamma> (insert v (vs \<union> vs')) e\<^sub>2 e\<^sub>2' t\<^sub>2 vs'' con\<^sub>2 \<Longrightarrow>
+    P \<Gamma> vs (App\<^sub>s e\<^sub>1 e\<^sub>2) (App\<^sub>s e\<^sub>1' e\<^sub>2') (Var v) (insert v (vs' \<union> vs'')) 
+      (con\<^sub>1 @ con\<^sub>2 @ [(t\<^sub>1, Arrow\<^sub>\<tau> t\<^sub>2 (Var v))])) \<Longrightarrow> 
+  P \<Gamma> vs e e' t vs' con"
   by (induction e arbitrary: \<Gamma> vs e' t vs' con) 
      (auto simp add: Let_def split: option.splits prod.splits)
 
+text \<open>Full typechecking is now easy. We generate our annotated expression, type term, and 
+constraints and then try to unify the constraint; if it fails, we fail, and if it succeeds, we 
+can use the unifying substitution to produce the final typed expression and type.\<close>
+
 fun typecheck :: "'a expr\<^sub>s \<rightharpoonup> ty expr\<^sub>s \<times> ty" where
   "typecheck e = (
-    let (e', t, vs, con) = typecheck' Map.empty {} e
-    in case unify con of 
-        Some sub \<Rightarrow> Some (map_expr\<^sub>s to_type (map_expr\<^sub>s (subst sub) e'), to_type (subst sub t))
+    let (e', \<tau>, vs, \<kappa>) = typecheck' Map.empty {} e
+    in case unify \<kappa> of 
+        Some \<sigma> \<Rightarrow> Some (map_expr\<^sub>s to_type (map_expr\<^sub>s (subst \<sigma>) e'), to_type (subst \<sigma> \<tau>))
       | None \<Rightarrow> None)"
 
 abbreviation erase :: "'a expr\<^sub>s \<Rightarrow> unit expr\<^sub>s" where
@@ -170,86 +191,74 @@ lemma [dest]: "erase e\<^sub>t = Lam\<^sub>s x u e \<Longrightarrow> \<exists>t 
 lemma [dest]: "erase e\<^sub>t = App\<^sub>s e\<^sub>1 e\<^sub>2 \<Longrightarrow> \<exists>e\<^sub>1' e\<^sub>2'. e\<^sub>t = App\<^sub>s e\<^sub>1' e\<^sub>2' \<and> e\<^sub>1 = erase e\<^sub>1'\<and> e\<^sub>2 = erase e\<^sub>2'"
   by (induction e\<^sub>t) simp_all
 
-lemma vars_expand: "typecheck' \<Gamma> vs e = (e', t, vs', con) \<Longrightarrow> vs \<subseteq> vs'"
+lemma [simp]: "typecheck' \<Gamma> vs e = (e', t, vs', con) \<Longrightarrow> finite vs \<Longrightarrow> finite vs'"
   by (induction e arbitrary: \<Gamma> vs e' t vs' con) 
-     (simp_all add: Let_def split: option.splits prod.splits, fastforce+)
+     (auto simp add: Let_def split: option.splits prod.splits)
 
-lemma [simp]: "typecheck' \<Gamma> vs e = (e', t, vs', con) \<Longrightarrow> finite vs' = finite vs"
-  by (induction e arbitrary: \<Gamma> vs e' t vs' con) 
-     (simp_all add: Let_def split: option.splits prod.splits)
-
-lemma [simp]: "typecheck' \<Gamma> vs e = (e', t', vs', con) \<Longrightarrow> finite vs \<Longrightarrow> tyvars\<^sub>s e' \<subseteq> vs' - vs"
-proof (induction rule: typecheck_induct)
-  case (Lam\<^sub>s \<Gamma> vs vs' con x u e\<^sub>1 e\<^sub>1' t' v)
-  moreover hence "insert v vs \<subseteq> vs'" by (metis vars_expand)
-  ultimately show ?case by auto
+lemma [simp]: "typecheck' \<Gamma> vs e = (e', t, vs', con) \<Longrightarrow> finite vs \<Longrightarrow> vs \<inter> vs' = {}"
+proof (induction e arbitrary: \<Gamma> vs e' t vs' con)
+  case (Lam\<^sub>s x u e)
+  let ?v = "fresh vs"
+  obtain e'' \<tau> vs'' \<kappa> where T: "typecheck' (\<Gamma>(x \<mapsto> Var ?v)) (insert ?v vs) e = (e'', \<tau>, vs'', \<kappa>)"
+    by (metis prod_cases4)
+  with Lam\<^sub>s have "e' = Lam\<^sub>s x (Var ?v) e'' \<and> t = Arrow\<^sub>\<tau> (Var ?v) \<tau> \<and> vs' = insert ?v vs'' \<and> 
+    con = \<kappa>" by (simp add: Let_def)
+  with Lam\<^sub>s T show ?case by fastforce
 next
-  case (App\<^sub>s \<Gamma> vs vs' e\<^sub>1 e\<^sub>2 v e\<^sub>1' t\<^sub>1 vs'' con\<^sub>1 e\<^sub>2' t\<^sub>2 con\<^sub>2)
-  moreover hence "insert v vs \<subseteq> vs''" by (metis vars_expand)
-  moreover from App\<^sub>s have "vs'' \<subseteq> vs'" by (metis vars_expand)
-  ultimately show ?case by auto
-qed simp_all
+  case (App\<^sub>s e\<^sub>1 e\<^sub>2)
+  let ?v = "fresh vs"
+  obtain e\<^sub>1' \<tau>\<^sub>1 vs\<^sub>1 \<kappa>\<^sub>1 where T1: "typecheck' \<Gamma> (insert ?v vs) e\<^sub>1 = (e\<^sub>1', \<tau>\<^sub>1, vs\<^sub>1, \<kappa>\<^sub>1)"
+    by (metis prod_cases4)
+  obtain e\<^sub>2' \<tau>\<^sub>2 vs\<^sub>2 \<kappa>\<^sub>2 where T2: "typecheck' \<Gamma> (insert ?v (vs \<union> vs\<^sub>1)) e\<^sub>2 = (e\<^sub>2', \<tau>\<^sub>2, vs\<^sub>2, \<kappa>\<^sub>2)"
+    by (metis prod_cases4)
+  with App\<^sub>s T1 have "e' = App\<^sub>s e\<^sub>1' e\<^sub>2' \<and> t = Var ?v \<and> vs' = insert ?v (vs\<^sub>1 \<union> vs\<^sub>2) \<and>
+    con = \<kappa>\<^sub>1 @ \<kappa>\<^sub>2 @ [(\<tau>\<^sub>1, Arrow\<^sub>\<tau> \<tau>\<^sub>2 (Var ?v))]" by (auto simp add: Let_def)
+  with App\<^sub>s T1 T2 show ?case by fastforce
+qed (simp_all split: option.splits)
+     
+lemma [simp]: "typecheck' \<Gamma> vs e = (e', t', vs', con) \<Longrightarrow> finite vs \<Longrightarrow> tyvars\<^sub>s e' \<subseteq> vs'"
+  by (induction rule: typecheck_induct) auto
 
 lemma [simp]: "typecheck' \<Gamma> vs e = (e', t', vs', con) \<Longrightarrow> x \<in> vs \<Longrightarrow> finite vs \<Longrightarrow> x \<notin> tyvars\<^sub>s e'"
 proof -
-  assume "typecheck' \<Gamma> vs e = (e', t', vs', con)"
-     and "finite vs"
-  hence "tyvars\<^sub>s e' \<subseteq> vs' - vs" by simp
+  assume T: "typecheck' \<Gamma> vs e = (e', t', vs', con)" and F: "finite vs"
+  hence "tyvars\<^sub>s e' \<subseteq> vs'" by simp
+  moreover from T F have "vs \<inter> vs' = {}" by simp
   moreover assume "x \<in> vs" 
   ultimately show "x \<notin> tyvars\<^sub>s e'" by auto
 qed
 
 lemma [simp]: "typecheck' \<Gamma> vs e = (e', t', vs', con) \<Longrightarrow> finite vs \<Longrightarrow> 
-  uvars t' \<subseteq> vs' - vs \<union> subst_vars \<Gamma>"
-proof (induction rule: typecheck_induct)
-  case (Lam\<^sub>s \<Gamma> vs vs' con x u e\<^sub>1 e\<^sub>1' t' v)
-  moreover hence "insert v vs \<subseteq> vs'" by (metis vars_expand)
-  ultimately show ?case by auto
-next
-  case (App\<^sub>s \<Gamma> vs vs' e\<^sub>1 e\<^sub>2 v e\<^sub>1' t\<^sub>1 vs'' con\<^sub>1 e\<^sub>2' t\<^sub>2 con\<^sub>2)
-  moreover hence "insert v vs \<subseteq> vs''" by (metis vars_expand)
-  moreover from App\<^sub>s have "vs'' \<subseteq> vs'" by (metis vars_expand)
-  ultimately show ?case by auto
-qed auto
+    uvars t' \<subseteq> vs' \<union> subst_vars \<Gamma>"
+  by (induction rule: typecheck_induct) auto
 
 lemma [simp]: "typecheck' \<Gamma> vs e = (e', t', vs', con) \<Longrightarrow> x \<in> vs \<Longrightarrow> finite vs \<Longrightarrow>
   x \<notin> subst_vars \<Gamma> \<Longrightarrow> x \<notin> uvars t'"
 proof -
-  assume "typecheck' \<Gamma> vs e = (e', t', vs', con)"
-     and "finite vs"
-  hence "uvars t' \<subseteq> vs' - vs \<union> subst_vars \<Gamma>" by simp
+  assume T: "typecheck' \<Gamma> vs e = (e', t', vs', con)" and F: "finite vs"
+  hence "uvars t' \<subseteq> vs' \<union> subst_vars \<Gamma>" by simp
+  moreover from T F have "vs \<inter> vs' = {}" by simp
   moreover assume "x \<in> vs" and "x \<notin> subst_vars \<Gamma>" 
   ultimately show "x \<notin> uvars t'" by auto
 qed
 
 lemma [simp]: "typecheck' \<Gamma> vs e = (e', t', vs', con) \<Longrightarrow> finite vs \<Longrightarrow> 
-  constr_vars con \<subseteq> vs' - vs \<union> subst_vars \<Gamma>"
-proof (induction rule: typecheck_induct)
-  case (Lam\<^sub>s \<Gamma> vs vs' con x u e\<^sub>1 e\<^sub>1' t' v)
-  moreover hence "insert v vs \<subseteq> vs'" by (metis vars_expand)
-  ultimately show ?case by auto
-next
+  constr_vars con \<subseteq> vs' \<union> subst_vars \<Gamma>"
+proof (induction rule: typecheck_induct) 
   case (App\<^sub>s \<Gamma> vs vs' e\<^sub>1 e\<^sub>2 v e\<^sub>1' t\<^sub>1 vs'' con\<^sub>1 e\<^sub>2' t\<^sub>2 con\<^sub>2)
-  moreover hence V1: "insert v vs \<subseteq> vs''" by (metis vars_expand)
-  moreover from App\<^sub>s have V2: "vs'' \<subseteq> vs'" by (metis vars_expand)
-  ultimately have V: "v \<in> vs' \<and> v \<notin> vs" by auto
-  from App\<^sub>s have "constr_vars con\<^sub>1 \<subseteq> vs'' - insert v vs \<union> subst_vars \<Gamma>" by simp
-  with V2 have C1: "constr_vars con\<^sub>1 \<subseteq> vs' - vs \<union> subst_vars \<Gamma>" by auto
-  from App\<^sub>s have "constr_vars con\<^sub>2 \<subseteq> vs' - vs'' \<union> subst_vars \<Gamma>" by simp
-  with V1 have C2: "constr_vars con\<^sub>2 \<subseteq> vs' - vs \<union> subst_vars \<Gamma>" by auto
-  from App\<^sub>s have "uvars t\<^sub>1 \<subseteq> vs'' - insert v vs \<union> subst_vars \<Gamma>" by simp
-  with V2 have T1: "uvars t\<^sub>1 \<subseteq> vs' - vs \<union> subst_vars \<Gamma>" by auto
-  from App\<^sub>s have "uvars t\<^sub>2 \<subseteq> vs' - vs'' \<union> subst_vars \<Gamma>" by simp
-  with V1 have "uvars t\<^sub>2 \<subseteq> vs' - vs \<union> subst_vars \<Gamma>" by auto
-  with V C1 C2 T1 show ?case by simp
-qed simp_all
+  hence "uvars t\<^sub>1 \<subseteq> vs' \<union> subst_vars \<Gamma>" by simp
+  moreover from App\<^sub>s have "uvars t\<^sub>2 \<subseteq> vs'' \<union> subst_vars \<Gamma>" by simp
+  ultimately have "uvars t\<^sub>1 \<subseteq> insert v (vs' \<union> vs'' \<union> subst_vars \<Gamma>) \<and> 
+    uvars t\<^sub>2 \<subseteq> insert v (vs' \<union> vs'' \<union> subst_vars \<Gamma>)" by auto
+  with App\<^sub>s show ?case by auto
+qed auto
 
 lemma [simp]: "typecheck' \<Gamma> vs e = (e', t', vs', con) \<Longrightarrow> x \<in> vs \<Longrightarrow> finite vs \<Longrightarrow>
   x \<notin> subst_vars \<Gamma> \<Longrightarrow> x \<notin> constr_vars con"
 proof -
-  assume "typecheck' \<Gamma> vs e = (e', t', vs', con)"
-     and "finite vs"
-  hence "constr_vars con \<subseteq> vs' - vs \<union> subst_vars \<Gamma>" by simp
+  assume T: "typecheck' \<Gamma> vs e = (e', t', vs', con)" and F: "finite vs"
+  hence "constr_vars con \<subseteq> vs' \<union> subst_vars \<Gamma>" by simp
+  moreover from T F have "vs \<inter> vs' = {}" by simp
   moreover assume "x \<in> vs" and "x \<notin> subst_vars \<Gamma>" 
   ultimately show "x \<notin> constr_vars con" by auto
 qed
@@ -278,12 +287,12 @@ next
   from Lam\<^sub>s have F: "fresh vs \<noteq> y" using fresh_is_fresh by blast
   obtain e'' tt' vs'' con' where T: "typecheck' (\<Gamma>(x \<mapsto> Var y, z \<mapsto> Var ?v)) (insert ?v vs) e = 
     (e'', tt', vs'', con')" by (metis prod_cases4)
+  with Lam\<^sub>s(2) have E: "e' = Lam\<^sub>s z (Var ?v) e'' \<and> tt = Arrow\<^sub>\<tau> (Var ?v) tt' \<and> vs' = insert ?v vs'' \<and> 
+    con' = con" by (simp only: typecheck'.simps Let_def split: prod.splits) simp
   show ?case
   proof (cases "x = z")
     case True
-    from T Lam\<^sub>s(2) have E: "e' = Lam\<^sub>s z (Var ?v) e'' \<and> tt = Arrow\<^sub>\<tau> (Var ?v) tt' \<and> 
-      vs'' = vs' \<and> con' = con" by (simp only: typecheck'.simps Let_def split: prod.splits) simp
-    from T True E have T': "typecheck' (\<Gamma>(z \<mapsto> Var ?v)) (insert ?v vs) e = (e'', tt', vs', con)" 
+    with T E have T': "typecheck' (\<Gamma>(z \<mapsto> Var ?v)) (insert ?v vs) e = (e'', tt', vs'', con)" 
       by simp
     from Lam\<^sub>s(4) F have "y \<notin> subst_vars (\<Gamma>(z \<mapsto> Var ?v))" 
       by (auto simp add: subst_vars_def ran_def)
@@ -294,16 +303,14 @@ next
   next
     case False
     from Lam\<^sub>s have "typecheck' (\<Gamma>(x \<mapsto> Var y)) vs (Lam\<^sub>s z u e) = (e', tt, vs', con)" by blast
-    with T have E: "e' = Lam\<^sub>s z (Var ?v) e'' \<and> tt = Arrow\<^sub>\<tau> (Var ?v) tt' \<and> vs'' = vs' \<and> 
-      con' = con" by (simp add: Let_def)
     from E T False have X: "typecheck' (\<Gamma>(z \<mapsto> Var ?v, x \<mapsto> Var y)) (insert ?v vs) e = 
-      (e'', tt', vs', con)" by (metis fun_upd_twist)
+      (e'', tt', vs'', con)" by (metis fun_upd_twist)
     have "subst_vars (\<Gamma>(z := None)) \<subseteq> subst_vars \<Gamma>" by simp
     with Lam\<^sub>s(4) F have "subst_vars (\<Gamma>(z \<mapsto> Var ?v)) \<subseteq> insert ?v vs - {y}" by fastforce
     with Lam\<^sub>s X have "typecheck' (\<Gamma>(z \<mapsto> Var ?v, x \<mapsto> t')) (insert ?v vs) e = 
-      (map_expr\<^sub>s (subst [y \<mapsto> t']) e'', subst [y \<mapsto> t'] tt', vs', constr_subst y t' con)" by blast
+      (map_expr\<^sub>s (subst [y \<mapsto> t']) e'', subst [y \<mapsto> t'] tt', vs'', constr_subst y t' con)" by blast
     with False have "typecheck' (\<Gamma>(x \<mapsto> t', z \<mapsto> Var ?v)) (insert ?v vs) e = 
-      (map_expr\<^sub>s (subst [y \<mapsto> t']) e'', subst [y \<mapsto> t'] tt', vs', constr_subst y t' con)" 
+      (map_expr\<^sub>s (subst [y \<mapsto> t']) e'', subst [y \<mapsto> t'] tt', vs'', constr_subst y t' con)" 
         by (metis fun_upd_twist)
     with E F have "typecheck' (\<Gamma>(x \<mapsto> t')) vs (Lam\<^sub>s z u e) =
       (map_expr\<^sub>s (subst [y \<mapsto> t']) e', subst [y \<mapsto> t'] tt, vs', constr_subst y t' con)" 
@@ -313,38 +320,37 @@ next
 next
   case (App\<^sub>s e1 e2)
   let ?v = "fresh vs"
-  obtain e\<^sub>1' t\<^sub>1 vs'' con\<^sub>1 where T1: "typecheck' (\<Gamma>(x \<mapsto> Var y)) (insert ?v vs) e1 = 
-    (e\<^sub>1', t\<^sub>1, vs'', con\<^sub>1)" by (metis prod_cases4)
-  moreover obtain e\<^sub>2' t\<^sub>2 vs''' con\<^sub>2 where T2: "typecheck' (\<Gamma>(x \<mapsto> Var y)) vs'' e2 = 
-    (e\<^sub>2', t\<^sub>2, vs''', con\<^sub>2)" by (metis prod_cases4)
+  obtain e\<^sub>1' \<tau>\<^sub>1 vs\<^sub>1 \<kappa>\<^sub>1 where T1: "typecheck' (\<Gamma>(x \<mapsto> Var y)) (insert ?v vs) e1 = 
+    (e\<^sub>1', \<tau>\<^sub>1, vs\<^sub>1, \<kappa>\<^sub>1)" by (metis prod_cases4)
+  moreover obtain e\<^sub>2' t\<^sub>2 vs\<^sub>2 \<kappa>\<^sub>2 where T2: "
+    typecheck' (\<Gamma>(x \<mapsto> Var y)) (insert ?v (vs \<union> vs\<^sub>1)) e2 = (e\<^sub>2', t\<^sub>2, vs\<^sub>2, \<kappa>\<^sub>2)" 
+      by (metis prod_cases4)
   moreover from App\<^sub>s have "typecheck' (\<Gamma>(x \<mapsto> Var y)) vs (App\<^sub>s e1 e2) = (e', tt, vs', con)" by blast
-  ultimately have E: "e' = App\<^sub>s e\<^sub>1' e\<^sub>2' \<and> tt = Var ?v \<and> vs''' = vs' \<and> 
-    con = con\<^sub>1 @ con\<^sub>2 @ [(t\<^sub>1, Arrow\<^sub>\<tau> t\<^sub>2 (Var ?v))]" by (auto simp add: Let_def)
-  from T1 have V: "vs \<subseteq> vs''" using vars_expand by blast
-  from App\<^sub>s V have A: "y \<in> vs''" by auto
-  from App\<^sub>s V have B: "subst_vars \<Gamma> \<subseteq> vs'' - {y}" by auto
-  from App\<^sub>s V have C: "uvars t' \<subseteq> vs'' - {y}" by auto
-  from App\<^sub>s T1 have D: "finite vs''" by simp
-  from App\<^sub>s T1 have T1': "typecheck' (\<Gamma>(x \<mapsto> t')) (insert ?v vs) e1 = 
-    (map_expr\<^sub>s (subst [y \<mapsto> t']) e\<^sub>1', subst [y \<mapsto> t'] t\<^sub>1, vs'', constr_subst y t' con\<^sub>1)" by blast
-  from App\<^sub>s T2 A B C D have T2': "typecheck' (\<Gamma>(x \<mapsto> t')) vs'' e2 = 
-    (map_expr\<^sub>s (subst [y \<mapsto> t']) e\<^sub>2', subst [y \<mapsto> t'] t\<^sub>2, vs''', constr_subst y t' con\<^sub>2)" by blast
-  from App\<^sub>s E T1' T2' have "typecheck' (\<Gamma>(x \<mapsto> t')) vs (App\<^sub>s e1 e2) = 
-    (map_expr\<^sub>s (subst [y \<mapsto> t']) e', subst [y \<mapsto> t'] tt, vs', constr_subst y t' con)" by (auto simp add: Let_def)
+  ultimately have E: "e' = App\<^sub>s e\<^sub>1' e\<^sub>2' \<and> tt = Var ?v \<and> vs' = insert ?v (vs\<^sub>1 \<union> vs\<^sub>2) \<and> 
+    con = \<kappa>\<^sub>1 @ \<kappa>\<^sub>2 @ [(\<tau>\<^sub>1, Arrow\<^sub>\<tau> t\<^sub>2 (Var ?v))]" by (auto simp add: Let_def)
+  moreover from App\<^sub>s T1 have "typecheck' (\<Gamma>(x \<mapsto> t')) (insert ?v vs) e1 =
+    (map_expr\<^sub>s (subst [y \<mapsto> t']) e\<^sub>1', subst [y \<mapsto> t'] \<tau>\<^sub>1, vs\<^sub>1, constr_subst y t' \<kappa>\<^sub>1)" by blast
+  moreover from App\<^sub>s T1 have "finite (insert ?v (vs \<union> vs\<^sub>1))" by simp
+  moreover with App\<^sub>s T2 have "typecheck' (\<Gamma>(x \<mapsto> t')) (insert ?v (vs \<union> vs\<^sub>1)) e2 =
+    (map_expr\<^sub>s (subst [y \<mapsto> t']) e\<^sub>2', subst [y \<mapsto> t'] t\<^sub>2, vs\<^sub>2, constr_subst y t' \<kappa>\<^sub>2)" by blast
+  moreover from App\<^sub>s have "y \<noteq> ?v" by auto
+  ultimately have "typecheck' (\<Gamma>(x \<mapsto> t')) vs (App\<^sub>s e1 e2) =
+    (map_expr\<^sub>s (subst [y \<mapsto> t']) e', subst [y \<mapsto> t'] tt, vs', constr_subst y t' con)" 
+      by (simp add: Let_def)
   thus ?case by blast
 qed auto
 
 lemma typecheck_fails' [simp]: "map_option to_type \<circ> \<Gamma> \<turnstile>\<^sub>t e\<^sub>t : t \<Longrightarrow> finite vs \<Longrightarrow> 
   subst_vars \<Gamma> \<subseteq> vs \<Longrightarrow> valid_ty_subst \<Gamma> \<Longrightarrow> typecheck' \<Gamma> vs (erase e\<^sub>t) = (e', tt, vs', con) \<Longrightarrow> 
   \<exists>s. map_expr\<^sub>s (eliminate_vars vs) (map_expr\<^sub>s (subst s) e') = map_expr\<^sub>s to_unifiable e\<^sub>t \<and> 
-  eliminate_vars vs (subst s tt) = to_unifiable t \<and> dom s = vs' - vs \<and> 
-  subst_vars s = {} \<and> s unifies\<^sub>\<kappa> eliminate_vars_constr vs con \<and> valid_ty_subst s \<and> idempotent s"
+  eliminate_vars vs (subst s tt) = to_unifiable t \<and> dom s = vs' \<and> subst_vars s = {} \<and> 
+  s unifies\<^sub>\<kappa> eliminate_vars_constr vs con \<and> valid_ty_subst s \<and> idempotent s"
 proof (induction "map_option to_type \<circ> \<Gamma>" e\<^sub>t t arbitrary: \<Gamma> vs e' tt vs' con rule: typing\<^sub>t.induct)
   case (tc\<^sub>t_lam x t\<^sub>1 e t\<^sub>2)
   let ?v = "fresh vs"
   obtain e'' t' vs'' con' where T: "typecheck' (\<Gamma>(x \<mapsto> Var ?v)) (insert ?v vs) (erase e) = 
     (e'', t', vs'', con')" by (metis prod_cases4)
-  with tc\<^sub>t_lam have E: "e' = Lam\<^sub>s x (Var ?v) e'' \<and> tt = Arrow\<^sub>\<tau> (Var ?v) t' \<and> vs'' = vs' \<and> 
+  with tc\<^sub>t_lam have E: "e' = Lam\<^sub>s x (Var ?v) e'' \<and> tt = Arrow\<^sub>\<tau> (Var ?v) t' \<and> vs' = insert ?v vs'' \<and> 
     con' = con" by (simp add: Let_def)
   from tc\<^sub>t_lam have "subst_vars \<Gamma> \<subseteq> insert ?v vs" by auto
   hence X: "subst_vars (\<Gamma>(x \<mapsto> to_unifiable t\<^sub>1)) \<subseteq> insert ?v vs" by simp
@@ -358,7 +364,7 @@ proof (induction "map_option to_type \<circ> \<Gamma>" e\<^sub>t t arbitrary: \<
     map_expr\<^sub>s (eliminate_vars (insert ?v vs)) (map_expr\<^sub>s (subst s) (map_expr\<^sub>s (subst [?v \<mapsto> to_unifiable t\<^sub>1]) e'')) = map_expr\<^sub>s to_unifiable e \<and> 
     eliminate_vars (insert ?v vs) (subst s (subst [?v \<mapsto> to_unifiable t\<^sub>1] t')) = to_unifiable t\<^sub>2 \<and>
     s unifies\<^sub>\<kappa> eliminate_vars_constr (insert ?v vs) (constr_subst ?v (to_unifiable t\<^sub>1) con') \<and> 
-    dom s = vs'' - insert ?v vs \<and> subst_vars s = {} \<and> valid_ty_subst s \<and> idempotent s" by meson
+    dom s = vs'' \<and> subst_vars s = {} \<and> valid_ty_subst s \<and> idempotent s" by meson
   from tc\<^sub>t_lam have "subst_vars (\<Gamma>(x \<mapsto> to_unifiable t\<^sub>1)) \<subseteq> vs" by simp
   moreover from tc\<^sub>t_lam have FV: "?v \<notin> vs" by simp
   ultimately have "?v \<notin> subst_vars (\<Gamma>(x \<mapsto> to_unifiable t\<^sub>1))" by blast
@@ -374,14 +380,13 @@ proof (induction "map_option to_type \<circ> \<Gamma>" e\<^sub>t t arbitrary: \<
   with S have "?v \<notin> tyvars\<^sub>s (map_expr\<^sub>s (subst (extend_subst ?v (to_unifiable t\<^sub>1) s)) e')" by auto
   with E S VCS have A: "map_expr\<^sub>s (eliminate_vars vs) (map_expr\<^sub>s (subst (extend_subst ?v (to_unifiable t\<^sub>1) s)) e') = 
     map_expr\<^sub>s to_unifiable (Lam\<^sub>s x t\<^sub>1 e)" by simp
-  from tc\<^sub>t_lam S have U: "?v \<notin> dom s" by auto
+  from tc\<^sub>t_lam T have "insert ?v vs \<inter> vs'' = {}" by simp
+  with S have U: "?v \<notin> dom s" by blast
   with S have B: "idempotent (extend_subst ?v (to_unifiable t\<^sub>1) s)" by simp
   from S E FV have "s unifies\<^sub>\<kappa> constr_subst ?v (to_unifiable t\<^sub>1) (eliminate_vars_constr vs con)" 
     by simp
   hence C: "extend_subst ?v (to_unifiable t\<^sub>1) s unifies\<^sub>\<kappa> eliminate_vars_constr vs con" by simp
-  from E TC have "insert ?v vs \<subseteq> vs'" by (metis vars_expand)
-  with tc\<^sub>t_lam have "insert ?v (vs' - insert ?v vs) = vs' - vs" by auto
-  with S E have D: "dom (extend_subst ?v (to_unifiable t\<^sub>1) s) = vs' - vs" by simp
+  from S E have D: "dom (extend_subst ?v (to_unifiable t\<^sub>1) s) = vs'" by simp
   have VS: "uvars (subst s (to_unifiable t\<^sub>1)) \<subseteq> uvars (to_unifiable t\<^sub>1) - dom s \<union> subst_vars s" 
     by (metis uvars_subst)
   from S U VS have F: "subst_vars (extend_subst ?v (to_unifiable t\<^sub>1) s) = {}" by auto
@@ -405,44 +410,47 @@ proof (induction "map_option to_type \<circ> \<Gamma>" e\<^sub>t t arbitrary: \<
 next
   case (tc\<^sub>t_app e\<^sub>1 t\<^sub>1 t\<^sub>2 e\<^sub>2)
   let ?v = "fresh vs"
-  obtain e\<^sub>1' t\<^sub>1' vs'' con\<^sub>1 where TC1: "typecheck' \<Gamma> (insert ?v vs) (erase e\<^sub>1) = 
-    (e\<^sub>1', t\<^sub>1', vs'', con\<^sub>1)" by (metis prod_cases4)
-  obtain e\<^sub>2' t\<^sub>2' vs''' con\<^sub>2 where TC2: "typecheck' \<Gamma> vs'' (erase e\<^sub>2) = (e\<^sub>2', t\<^sub>2', vs''', con\<^sub>2)"
-    by (metis prod_cases4)
-  with tc\<^sub>t_app TC1 have E: "e' = App\<^sub>s e\<^sub>1' e\<^sub>2' \<and> tt = Var ?v \<and> vs''' = vs' \<and> 
+  obtain e\<^sub>1' t\<^sub>1' vs\<^sub>1 con\<^sub>1 where TC1: "typecheck' \<Gamma> (insert ?v vs) (erase e\<^sub>1) = 
+    (e\<^sub>1', t\<^sub>1', vs\<^sub>1, con\<^sub>1)" by (metis prod_cases4)
+  obtain e\<^sub>2' t\<^sub>2' vs\<^sub>2 con\<^sub>2 where TC2: "typecheck' \<Gamma> (insert ?v (vs \<union> vs\<^sub>1)) (erase e\<^sub>2) = 
+    (e\<^sub>2', t\<^sub>2', vs\<^sub>2, con\<^sub>2)" by (metis prod_cases4)
+  with tc\<^sub>t_app TC1 have E: "e' = App\<^sub>s e\<^sub>1' e\<^sub>2' \<and> tt = Var ?v \<and> vs' = insert ?v (vs\<^sub>1 \<union> vs\<^sub>2) \<and> 
     con = con\<^sub>1 @ con\<^sub>2 @ [(t\<^sub>1', Arrow\<^sub>\<tau> t\<^sub>2' (Var ?v))]" by (auto simp add: Let_def)
   from tc\<^sub>t_app have "subst_vars \<Gamma> \<subseteq> insert ?v vs" by auto
   with tc\<^sub>t_app TC1 obtain s\<^sub>1 where S1: "
     map_expr\<^sub>s (eliminate_vars (insert ?v vs)) (map_expr\<^sub>s (subst s\<^sub>1) e\<^sub>1') = map_expr\<^sub>s to_unifiable e\<^sub>1 \<and> 
     eliminate_vars (insert ?v vs) (subst s\<^sub>1 t\<^sub>1') = to_unifiable (Arrow t\<^sub>1 t\<^sub>2) \<and> 
-    dom s\<^sub>1 = vs'' - insert ?v vs \<and> subst_vars s\<^sub>1 = {} \<and> 
+    dom s\<^sub>1 = vs\<^sub>1 \<and> subst_vars s\<^sub>1 = {} \<and> 
     s\<^sub>1 unifies\<^sub>\<kappa> eliminate_vars_constr (insert ?v vs) con\<^sub>1 \<and> valid_ty_subst s\<^sub>1 \<and> idempotent s\<^sub>1" 
-      by fastforce
-  from TC1 have V1: "insert ?v vs \<subseteq> vs''" by (metis vars_expand)
-  from TC2 E have V2: "vs'' \<subseteq> vs'" by (metis vars_expand)
-  with tc\<^sub>t_app V1 have Y: "subst_vars \<Gamma> \<subseteq> vs''" by auto
-  with tc\<^sub>t_app TC1 TC2 Y obtain s\<^sub>2 where S2: "map_expr\<^sub>s (eliminate_vars vs'') (map_expr\<^sub>s (subst s\<^sub>2) e\<^sub>2') = map_expr\<^sub>s to_unifiable e\<^sub>2 \<and> 
-    eliminate_vars vs'' (subst s\<^sub>2 t\<^sub>2') = to_unifiable t\<^sub>1 \<and> dom s\<^sub>2 = vs''' - vs'' \<and> subst_vars s\<^sub>2 = {} \<and> 
-    s\<^sub>2 unifies\<^sub>\<kappa> eliminate_vars_constr vs'' con\<^sub>2 \<and> valid_ty_subst s\<^sub>2 \<and> idempotent s\<^sub>2" by fastforce
+    by fastforce
+  from tc\<^sub>t_app TC1 TC2 have FVS: "finite (insert ?v (vs \<union> vs\<^sub>1))" by simp
+  from tc\<^sub>t_app have "subst_vars \<Gamma> \<subseteq> insert ?v (vs \<union> vs\<^sub>1)" by auto
+  with tc\<^sub>t_app TC2 FVS obtain s\<^sub>2 where S2: "
+    map_expr\<^sub>s (eliminate_vars (insert ?v (vs \<union> vs\<^sub>1))) (map_expr\<^sub>s (subst s\<^sub>2) e\<^sub>2') = 
+      map_expr\<^sub>s to_unifiable e\<^sub>2 \<and> 
+    eliminate_vars (insert ?v (vs \<union> vs\<^sub>1)) (subst s\<^sub>2 t\<^sub>2') = to_unifiable t\<^sub>1 \<and> dom s\<^sub>2 = vs\<^sub>2 \<and> subst_vars s\<^sub>2 = {} \<and> 
+    s\<^sub>2 unifies\<^sub>\<kappa> eliminate_vars_constr (insert ?v (vs \<union> vs\<^sub>1)) con\<^sub>2 \<and> valid_ty_subst s\<^sub>2 \<and> idempotent s\<^sub>2" 
+      by presburger
   from tc\<^sub>t_app have FV: "?v \<notin> vs" by simp
-  from S1 S2 have DSS: "dom s\<^sub>1 \<inter> dom s\<^sub>2 = {}" by auto
+  from tc\<^sub>t_app TC1 have VVS1: "insert ?v vs \<inter> vs\<^sub>1 = {}" by simp
+  moreover from tc\<^sub>t_app TC1 TC2 have VVS2: "insert ?v (vs \<union> vs\<^sub>1) \<inter> vs\<^sub>2 = {}" by simp
+  ultimately have VVS: "?v \<notin> vs\<^sub>1 \<union> vs\<^sub>2" by simp
+  from VVS2 S1 S2 have DSS: "dom s\<^sub>1 \<inter> dom s\<^sub>2 = {}" by auto
   from tc\<^sub>t_app TC1 S1 have "valid_ty_term t\<^sub>1' \<and> valid_ty_subst s\<^sub>1" by auto
   hence VTS1: "valid_ty_term (subst s\<^sub>1 t\<^sub>1')" by simp
   from tc\<^sub>t_app TC2 S2 have "valid_ty_term t\<^sub>2' \<and> valid_ty_subst s\<^sub>2" by auto
   hence VTS2: "valid_ty_term (subst s\<^sub>2 t\<^sub>2')" by simp
   let ?s = "extend_subst ?v (to_unifiable t\<^sub>2) (combine_subst s\<^sub>1 s\<^sub>2)"
-  from S1 have D1: "dom s\<^sub>1 = vs'' - insert ?v vs" by simp
-  from S2 E have D2: "dom s\<^sub>2 = vs' - vs''" by simp
-  with V1 V2 D1 have D3: "dom (combine_subst s\<^sub>1 s\<^sub>2) = vs' - insert ?v vs" by auto
-  with FV V1 V2 have A: "dom ?s = vs' - vs" by auto
+  from S1 S2 have D3: "dom (combine_subst s\<^sub>1 s\<^sub>2) = vs\<^sub>1 \<union> vs\<^sub>2" by auto
+  with FV E have A: "dom ?s = vs'" by simp
   from tc\<^sub>t_app have VG: "?v \<notin> subst_vars \<Gamma>" by auto 
   with tc\<^sub>t_app TC1 have VE1: "?v \<notin> tyvars\<^sub>s e\<^sub>1'" by simp
-  from tc\<^sub>t_app TC1 TC2 V1 VG have VE2: "?v \<notin> tyvars\<^sub>s e\<^sub>2'" by simp
-  from tc\<^sub>t_app TC1 have "tyvars\<^sub>s e\<^sub>1' \<subseteq> vs'' - insert ?v vs" by simp
-  with D2 have HV: "dom s\<^sub>2 \<inter> tyvars\<^sub>s e\<^sub>1' = {}" by auto
-  from tc\<^sub>t_app E TC1 TC2 have HV2: "tyvars\<^sub>s e\<^sub>2' \<subseteq> vs' - vs''" by simp
+  from tc\<^sub>t_app TC1 TC2 VG have VE2: "?v \<notin> tyvars\<^sub>s e\<^sub>2'" by simp
+  from tc\<^sub>t_app TC1 have "tyvars\<^sub>s e\<^sub>1' \<subseteq> vs\<^sub>1" by simp
+  with S1 S2 DSS have HV: "dom s\<^sub>2 \<inter> tyvars\<^sub>s e\<^sub>1' = {}" by blast
+  from tc\<^sub>t_app E TC1 TC2 have HV2: "tyvars\<^sub>s e\<^sub>2' \<subseteq> vs\<^sub>2" by simp
   have "tyvars\<^sub>s (map_expr\<^sub>s (subst s\<^sub>2) e\<^sub>2') \<subseteq> tyvars\<^sub>s e\<^sub>2' - dom s\<^sub>2 \<union> subst_vars s\<^sub>2" by simp
-  with D2 S2 HV2 have HVS2: "tyvars\<^sub>s (map_expr\<^sub>s (subst s\<^sub>2) e\<^sub>2') = {}" by auto
+  with S2 HV2 have HVS2: "tyvars\<^sub>s (map_expr\<^sub>s (subst s\<^sub>2) e\<^sub>2') = {}" by auto
   have "tyvars\<^sub>s (map_expr\<^sub>s (subst s\<^sub>1) e\<^sub>1') \<subseteq> tyvars\<^sub>s e\<^sub>1' - dom s\<^sub>1 \<union> subst_vars s\<^sub>1" by simp
   with VE1 S1 have "?v \<notin> tyvars\<^sub>s (map_expr\<^sub>s (subst s\<^sub>1) e\<^sub>1')" by blast
   with S1 HV have "map_expr\<^sub>s (eliminate_vars vs) (map_expr\<^sub>s (subst s\<^sub>1) (map_expr\<^sub>s (subst s\<^sub>2) e\<^sub>1')) = 
@@ -457,53 +465,45 @@ next
     map_expr\<^sub>s (eliminate_vars vs) (map_expr\<^sub>s (subst ?s) e\<^sub>2') = map_expr\<^sub>s to_unifiable e\<^sub>2" by simp
   hence B: "map_expr\<^sub>s (eliminate_vars vs) (map_expr\<^sub>s (subst ?s) (App\<^sub>s e\<^sub>1' e\<^sub>2')) = map_expr\<^sub>s to_unifiable (App\<^sub>s e\<^sub>1 e\<^sub>2)" by simp
   have C: "eliminate_vars vs (subst ?s (Var ?v)) = to_unifiable t\<^sub>2" by simp
-  from S1 S2 DSS D3 have D: "subst_vars ?s = {}" by auto
+  from S1 S2 DSS VVS D3 have D: "subst_vars ?s = {}" by simp
   from S1 S2 have VCS: "?v \<notin> subst_vars s\<^sub>1 \<and> ?v \<notin> subst_vars s\<^sub>2" by auto
-  from D2 S1 V1 have D2S1: "dom s\<^sub>2 \<inter> subst_vars s\<^sub>1 = {}" by auto
+  from S1 S2 have D2S1: "dom s\<^sub>2 \<inter> subst_vars s\<^sub>1 = {}" by auto
   from tc\<^sub>t_app TC1 VG have "?v \<notin> constr_vars con\<^sub>1" by simp
-  with S1 S2 DSS D3 D2S1 have UC1: "?s unifies\<^sub>\<kappa> eliminate_vars_constr vs con\<^sub>1" by simp
-  from V1 V2 have VVS': "vs \<subseteq> vs''" by simp
-  from tc\<^sub>t_app TC1 TC2 E have "constr_vars con\<^sub>2 \<subseteq> vs' - vs'' \<union> subst_vars \<Gamma>" by simp
-  with tc\<^sub>t_app have "constr_vars con\<^sub>2 \<inter> vs'' \<subseteq> vs" by auto
-  with S2 VVS' have "s\<^sub>2 unifies\<^sub>\<kappa> eliminate_vars_constr vs con\<^sub>2" 
-    by (metis partial_typeify_constr_reduce_subset)
-  with S1 S2 DSS D3 have UC2: "?s unifies\<^sub>\<kappa> eliminate_vars_constr vs con\<^sub>2" by simp
-  from tc\<^sub>t_app TC1 have UV1: "uvars t\<^sub>1' \<subseteq> vs'' - insert ?v vs \<union> subst_vars \<Gamma>" by simp
-  with VG have VT1: "?v \<notin> uvars t\<^sub>1'" by auto
-  from tc\<^sub>t_app D2 V1 UV1 have DU1: "dom s\<^sub>2 \<inter> uvars t\<^sub>1' = {}" by auto
-  from tc\<^sub>t_app TC1 TC2 E have UV2: "uvars t\<^sub>2' \<subseteq> vs' - vs'' \<union> subst_vars \<Gamma>" by simp
-  with VG V1 have VT2: "?v \<notin> uvars t\<^sub>2'" by auto
+  with VVS S1 S2 DSS D2S1 have UC1: "?s unifies\<^sub>\<kappa> eliminate_vars_constr vs con\<^sub>1" by simp  
+  from tc\<^sub>t_app TC1 TC2 E have "constr_vars con\<^sub>2 \<subseteq> vs\<^sub>2 \<union> subst_vars \<Gamma>" by simp
+  with tc\<^sub>t_app VVS2 have CV2: "constr_vars con\<^sub>2 \<inter> vs\<^sub>1 \<subseteq> vs" by auto
+  from tc\<^sub>t_app TC1 TC2 VG have "?v \<notin> constr_vars con\<^sub>2" by simp
+  with CV2 VVS S1 S2 DSS have UC2: "?s unifies\<^sub>\<kappa> eliminate_vars_constr vs con\<^sub>2" by simp
+  from tc\<^sub>t_app TC1 have UV1: "uvars t\<^sub>1' \<subseteq> vs\<^sub>1 \<union> subst_vars \<Gamma>" by simp
+  with VG VVS have VT1: "?v \<notin> uvars t\<^sub>1'" by auto
+  from DSS VVS2 have "vs\<^sub>2 \<inter> (vs\<^sub>1 \<union> vs) = {}" by blast
+  with tc\<^sub>t_app(6) S2 UV1 have DU1: "dom s\<^sub>2 \<inter> uvars t\<^sub>1' = {}" by blast
+  from tc\<^sub>t_app TC1 TC2 E have UV2: "uvars t\<^sub>2' \<subseteq> vs\<^sub>2 \<union> subst_vars \<Gamma>" by simp
+  with VG VVS have VT2: "?v \<notin> uvars t\<^sub>2'" by auto
   have "uvars (subst s\<^sub>1 t\<^sub>1') \<subseteq> uvars t\<^sub>1' - dom s\<^sub>1 \<union> subst_vars s\<^sub>1" by simp
-  with S1 D1 UV1 have "uvars (subst s\<^sub>1 t\<^sub>1') \<subseteq> 
-    (vs'' - insert ?v vs \<union> subst_vars \<Gamma>) - (vs'' - insert ?v vs) \<union> {}" by auto
-  with tc\<^sub>t_app(6) have "uvars (subst s\<^sub>1 t\<^sub>1') \<subseteq> vs'' - insert ?v vs \<union> vs - (vs'' - insert ?v vs)" 
+  with S1 UV1 have "uvars (subst s\<^sub>1 t\<^sub>1') \<subseteq> 
+    (vs\<^sub>1 - insert ?v vs \<union> subst_vars \<Gamma>) - (vs\<^sub>1 - insert ?v vs) \<union> {}" by auto
+  with tc\<^sub>t_app(6) have "uvars (subst s\<^sub>1 t\<^sub>1') \<subseteq> vs\<^sub>1 - insert ?v vs \<union> vs - (vs\<^sub>1 - insert ?v vs)" 
     by auto
   hence US1: "uvars (subst s\<^sub>1 t\<^sub>1') \<subseteq> vs" by auto
-  have US2: "uvars (subst s\<^sub>2 t\<^sub>2') \<subseteq> uvars t\<^sub>2' - dom s\<^sub>2 \<union> subst_vars s\<^sub>2" by simp
-  with S2 D2 UV2 have "uvars (subst s\<^sub>2 t\<^sub>2') \<subseteq> (vs' - vs'' \<union> subst_vars \<Gamma>) - (vs' - vs'') \<union> {}" 
-    by auto
-  with tc\<^sub>t_app(6) have "uvars (subst s\<^sub>2 t\<^sub>2') \<subseteq> vs' - vs'' \<union> vs - (vs' - vs'')" by auto
-  hence US2: "uvars (subst s\<^sub>2 t\<^sub>2') \<subseteq> vs" by auto
-  have "(vs'' - insert ?v vs) \<inter> ((vs' - vs'' \<union> vs) - (vs' - vs'') \<union> vs) = {}" by auto
-  with tc\<^sub>t_app have "(vs'' - insert ?v vs) \<inter> ((vs' - vs'' \<union> subst_vars \<Gamma>) - (vs' - vs'') \<union> vs) = {}" 
-    by auto
-  with S2 D2 UV2 have "(vs'' - insert ?v vs) \<inter> (uvars t\<^sub>2' - dom s\<^sub>2 \<union> subst_vars s\<^sub>2) = {}" by auto
-  with D1 US2 have DU2: "dom s\<^sub>1 \<inter> uvars (subst s\<^sub>2 t\<^sub>2') = {}" by fast
-  from D1 have DSV1: "dom s\<^sub>1 \<inter> vs = {}" by auto
-  from D2 V1 have DSV2: "dom s\<^sub>2 \<inter> vs = {}" by auto
+  have "uvars (subst s\<^sub>2 t\<^sub>2') \<subseteq> uvars t\<^sub>2' - dom s\<^sub>2 \<union> subst_vars s\<^sub>2" by simp
+  with tc\<^sub>t_app(6) S2 UV2 have US2: "uvars (subst s\<^sub>2 t\<^sub>2') \<subseteq> vs" by blast
+  with S1 VVS1 have DU2: "dom s\<^sub>1 \<inter> uvars (subst s\<^sub>2 t\<^sub>2') = {}" by auto
+  from S1 VVS1 have DSV1: "dom s\<^sub>1 \<inter> vs = {}" by auto
+  from S2 VVS2 have DSV2: "dom s\<^sub>2 \<inter> vs = {}" by auto
   from S1 obtain tt1 tt2 where SS1: "subst s\<^sub>1 t\<^sub>1' = Arrow\<^sub>\<tau> tt1 tt2 \<and> 
     eliminate_vars (insert ?v vs) tt1 = to_unifiable t\<^sub>1 \<and> 
     eliminate_vars (insert ?v vs) tt2 = to_unifiable t\<^sub>2" by auto
   from US1 SS1 have "uvars tt1 \<subseteq> vs \<and> uvars tt2 \<subseteq> vs" by simp
   with FV SS1 have PT1: "eliminate_vars vs tt1 = to_unifiable t\<^sub>1 \<and> 
     eliminate_vars vs tt2 = to_unifiable t\<^sub>2" by force
-  from US2 have "uvars (subst s\<^sub>2 t\<^sub>2') \<inter> vs'' \<subseteq> vs" by auto
-  with S2 VVS' have "eliminate_vars vs (subst s\<^sub>2 t\<^sub>2') = to_unifiable t\<^sub>1"
-    by (metis partial_typeify_reduce_subset)
+  from US2 have USV21: "uvars (subst s\<^sub>2 t\<^sub>2') \<inter> vs\<^sub>1 \<subseteq> vs" by auto
+  from US2 FV have "?v \<notin> uvars (subst s\<^sub>2 t\<^sub>2')" by auto
+  with S2 USV21 have "eliminate_vars vs (subst s\<^sub>2 t\<^sub>2') = to_unifiable t\<^sub>1" by simp
   with FV UC1 UC2 S1 S2 DSV1 DSV2 VT1 VT2 DU1 DU2 SS1 PT1 have F: "
     ?s unifies\<^sub>\<kappa> eliminate_vars_constr vs (con\<^sub>1 @ con\<^sub>2 @ [(t\<^sub>1', Arrow\<^sub>\<tau> t\<^sub>2' (Var ?v))])" 
-      by (simp add: expand_extend_subst)
-  from DSS VCS V1 D1 D2 S1 S2 D2S1 have G: "idempotent ?s" by simp
+    by (simp add: expand_extend_subst)
+  from S1 S2 DSS VVS D3 have G: "idempotent ?s" by simp
   from S1 S2 have "valid_ty_subst ?s" by simp
   with E A B C D F G show ?case by blast
 qed auto
@@ -518,7 +518,7 @@ proof
   have Z: "subst_vars Map.empty \<subseteq> {}" by simp
   have "valid_ty_subst Map.empty \<and> finite {}" by simp
   with X Y Z have "\<exists>s. map_expr\<^sub>s (eliminate_vars {}) (map_expr\<^sub>s (subst s) e') = map_expr\<^sub>s to_unifiable e\<^sub>t \<and> 
-    eliminate_vars {} (subst s tt) = to_unifiable t \<and> dom s = vs' - {} \<and> subst_vars s = {} \<and> 
+    eliminate_vars {} (subst s tt) = to_unifiable t \<and> dom s = vs' \<and> subst_vars s = {} \<and> 
     s unifies\<^sub>\<kappa> eliminate_vars_constr {} con \<and> valid_ty_subst s \<and> idempotent s" 
     using typecheck_fails' by blast
   then obtain s where "s unifies\<^sub>\<kappa> eliminate_vars_constr {} con \<and> idempotent s" by blast
